Cleanup old crypto definitions.

crypto.v
@@ -113,132 +113,27 @@ Definition atomic t :=
 
 Context `{!heapG Σ}.
 
-Definition term_data : Type := gmap term (level * gname * gname).
-
-Global Instance term_data_inhabited : Inhabited term_data.
-Proof. apply _. Qed.
-
-Definition term_data' : Type :=
-  gmap term (agree level) *
-  gmap term (agree gname) *
-  gmap term (agree gname).
-
-Canonical term_data'UR :=
-  (fun (sT : ucmraT) (f : term_data' -> sT) => sT) _ (fun x => x).
-
-Definition to_term_data' (td : term_data) : term_data'UR :=
-  (fmap (fun '(lvl, _    , _)     => to_agree lvl)     td,
-   fmap (fun '(_  , γ_pub, _) => to_agree γ_pub)       td,
-   fmap (fun '(_  , _    , γ_meta) => to_agree γ_meta) td).
-
 Class cryptoG := CryptoG {
-  crypto_inG :> inG Σ (authUR term_data'UR);
   crypto_pub_inG :> savedPredG Σ term;
-  crypto_meta_inG :> inG Σ (namespace_mapR (agreeR positiveO));
-  crypto_pred_inG :> savedPredG Σ (term * term);
-  crypto_name : gname;
-  crypto_inv_name : gname;
+  crypto_enc_inG :> savedPredG Σ (term * term);
+  crypto_enc_name : gname;
 }.
 
 Context `{!cryptoG}.
 
-Global Instance cryptoG_authG : authG Σ term_data'UR := @AuthG _ _ _ _.
-
-Implicit Types d : level * gname * gname.
-Implicit Types td : term_data.
-
-Definition crypto_own (td : term_data'UR) :=
-  auth_own crypto_name td.
-
-Definition crypto_meta_name t γm : iProp :=
-  crypto_own (∅, ∅, {[t := to_agree γm]}).
-
-Global Instance crypto_meta_name_persistent t γm :
-  Persistent (crypto_meta_name t γm).
-Proof.
-rewrite /crypto_meta_name /crypto_own; by apply _.
-Qed.
-
-Lemma crypto_meta_name_agree t γm1 γm2 :
-  crypto_meta_name t γm1 -∗
-  crypto_meta_name t γm2 -∗
-  ⌜γm1 = γm2⌝.
-Proof.
-iIntros "own1 own2".
-iPoseProof (own_valid_2 with "own1 own2") as "#valid".
-rewrite auth_validI /= -!pair_op !uPred.prod_validI /=.
-iDestruct "valid" as "(_ & #valid)".
-rewrite singleton_op gmap_validI.
-iSpecialize ("valid" $! t); rewrite lookup_singleton.
-rewrite uPred.option_validI agree_validI agree_equivI.
-by iRewrite "valid".
-Qed.
-
-Definition crypto_meta_token t E : iProp :=
-  ∃ γm, crypto_meta_name t γm ∗ own γm (namespace_map_token E).
-
-Definition crypto_meta `{Countable A} t N (x : A) : iProp :=
-  ∃ γm, crypto_meta_name t γm ∗
-        own γm (namespace_map_data N (to_agree (encode x))).
-
-Global Instance crypto_meta_persistent `{Countable A} t N (x : A) :
-  Persistent (crypto_meta t N x).
-Proof. apply _. Qed.
-
-Lemma crypto_meta_agree `{Countable A} t N (x1 x2 : A) :
-  crypto_meta t N x1 -∗
-  crypto_meta t N x2 -∗
-  ⌜x1 = x2⌝.
-Proof.
-iDestruct 1 as (γm1) "[#meta1 #own1]".
-iDestruct 1 as (γm2) "[#meta2 #own2]".
-iPoseProof (crypto_meta_name_agree with "meta2 meta1") as "->".
-iPoseProof (own_valid_2 with "own1 own2") as "%valid".
-move: valid; rewrite -namespace_map_data_op namespace_map_data_valid.
-move=> /agree_op_invL'. naive_solver.
-Qed.
-
-Lemma crypto_meta_set `{Countable A} E t (x : A) (N : namespace) :
-  ↑N ⊆ E →
-  crypto_meta_token t E ==∗
-  crypto_meta t N x.
-Proof.
-iIntros (?) "token"; iDestruct "token" as (γ) "[own token]".
-iMod (own_update with "token").
-  by eapply (namespace_map_alloc_update _ _ (to_agree (encode x))) => //.
-by iModIntro; iExists γ; iSplit.
-Qed.
-
-Lemma crypto_meta_meta_token `{Countable A} t (x : A) N E :
-  ↑N ⊆ E →
-  crypto_meta_token t E -∗
-  crypto_meta t N x -∗
-  False.
-Proof.
-iIntros (sub) "Htoken #Hmeta1".
-pose (X := {[encode x]} : gset positive).
-iMod (crypto_meta_set _ (fresh X) with "Htoken") as "#Hmeta2"=> //.
-iAssert (crypto_meta t N (encode x)) as "Hmeta1'".
-  by rewrite {1 3}/crypto_meta.
-iPoseProof (crypto_meta_agree with "Hmeta1' Hmeta2") as "%e"; iPureIntro.
-assert (contra : encode x ∈ X). { by apply/elem_of_singleton. }
-destruct (is_fresh X); by rewrite -e.
-Qed.
-
-Definition crypto_inv_token E : iProp :=
-  own crypto_inv_name (namespace_map_token E).
-
-Definition crypto_inv_meta N Φ : iProp :=
-  ∃ γ, own crypto_inv_name (namespace_map_data N (to_agree γ)) ∧
+Definition crypto_enc N Φ : iProp :=
+  ∃ γ, own crypto_enc_name (namespace_map_data N (to_agree γ)) ∧
        saved_pred_own γ (fun '(k, t) => Φ k t).
 
-Global Instance crypto_inv_meta_persistent N Φ :
-  Persistent (crypto_inv_meta N Φ).
+Definition crypto_enc_token E :=
+  own crypto_enc_name (namespace_map_token E).
+
+Global Instance crypto_enc_persistent N Φ : Persistent (crypto_enc N Φ).
 Proof. apply _. Qed.
 
-Lemma crypto_inv_meta_agree k t N Φ1 Φ2 :
-  crypto_inv_meta N Φ1 -∗
-  crypto_inv_meta N Φ2 -∗
+Lemma crypto_enc_agree k t N Φ1 Φ2 :
+  crypto_enc N Φ1 -∗
+  crypto_enc N Φ2 -∗
   ▷ (Φ1 k t ≡ Φ2 k t).
 Proof.
 iDestruct 1 as (γm1) "[#meta1 #own1]".
@@ -249,10 +144,10 @@ move=> /agree_op_invL' ->.
 by iApply (saved_pred_agree _ _ _ (k, t) with "own1 own2").
 Qed.
 
-Lemma crypto_inv_meta_set E Φ N :
+Lemma crypto_enc_set E Φ N :
   ↑N ⊆ E →
-  crypto_inv_token E ==∗
-  crypto_inv_meta N Φ.
+  crypto_enc_token E ==∗
+  crypto_enc N Φ.
 Proof.
 iIntros (?) "token".
 iMod (saved_pred_alloc (λ '(k, t), Φ k t)) as (γ) "own".
@@ -262,38 +157,48 @@ by iModIntro; iExists γ; iSplit.
 Qed.
 
 Definition enc_inv k t : iProp :=
-  ∃ N t' Φ, ⌜t = Spec.tag N t'⌝ ∧ crypto_inv_meta N Φ ∧ □ Φ k t'.
+  ∃ N t' Φ, ⌜t = Spec.tag N t'⌝ ∧ crypto_enc N Φ ∧ □ Φ k t'.
 
 Global Instance enc_inv_persistent k t : Persistent (enc_inv k t).
 Proof. by apply _. Qed.
 
 Lemma enc_inv_elim k N t Φ :
   enc_inv k (Spec.tag N t) -∗
-  crypto_inv_meta N Φ -∗
+  crypto_enc N Φ -∗
   □ ▷ Φ k t.
 Proof.
 iDestruct 1 as (N' t' Φ') "(%t_t' & #HΦ' & #inv)"; iIntros "#HΦ".
 case/Spec.tag_inj: t_t' => <- <-.
-iPoseProof (crypto_inv_meta_agree k t with "HΦ HΦ'") as "e".
+iPoseProof (crypto_enc_agree k t with "HΦ HΦ'") as "e".
 by iIntros "!> !>"; iRewrite "e".
 Qed.
 
-Definition publish_pred a (P : term → iProp) : iProp :=
+Definition nonce_pred a (P : term → iProp) : iProp :=
   ∃ γ, meta a (cryptoN.@"nonce") γ ∧ saved_pred_own γ P.
 
-Global Instance Persistent_publish_pred a (P : term → iProp) :
-  Persistent (publish_pred a P).
+Global Instance Persistent_nonce_pred a (P : term → iProp) :
+  Persistent (nonce_pred a P).
 Proof. apply _. Qed.
 
+Lemma nonce_pred_set a (P : term → iProp) :
+  meta_token a (↑cryptoN.@"nonce") ==∗
+  nonce_pred a P.
+Proof.
+iIntros "token".
+iMod (saved_pred_alloc P) as (γ) "#HP".
+iMod (meta_set _ a γ with "token") as "#meta"; eauto.
+by iModIntro; iExists γ; eauto.
+Qed.
+
 Definition declared_nonce a : iProp :=
-  ∃ (P : term → iProp), publish_pred a P.
+  ∃ (P : term → iProp), nonce_pred a P.
 
 Global Instance Persistent_declared_nonce a :
   Persistent (declared_nonce a).
 Proof. apply _. Qed.
 
 Definition published a t : iProp :=
-  ∃ (P : term → iProp), publish_pred a P ∧ □ P t.
+  ∃ (P : term → iProp), nonce_pred a P ∧ □ P t.
 
 Global Instance Persistent_published a t :
   Persistent (published a t).
@@ -304,49 +209,6 @@ Definition sterm t : iProp :=
 
 Global Instance Persistent_sterm t : Persistent (sterm t).
 Proof. apply _. Qed.
-
-(*
-Inductive derive (T : gset term) (t : term) : Prop :=
-| DIn
-  of t ∈ T
-: derive T t
-
-| DInt n
-  of t = TInt n
-: derive T t
-
-| DPair t1 t2
-  of t = TPair t1 t2
-  &  derive T t1
-  &  derive T t2
-: derive T t
-
-| DKey kt t'
-  of t = TKey kt t'
-  &  derive T t'
-: derive T t
-
-| DEnc k t'
-  of t = TEnc k t'
-  &  derive T (TKey Enc k)
-  &  derive T t'
-: derive T t
-
-| DHash t'
-  of t = THash t'
-  &  derive T t'
-: derive T t
-
-| DExp0 t'
-  of t = TExp t' []
-  &  derive T t'
-
-| DExp1 t1 ts1 t2
-  of t = TExp t1 (t2 :: ts1)
-  &  derive T (TExp t1 ts1)
-  &  derive T t2
-: derive T t.
-*)
 
 Inductive decompose (T : gset term) (t : term) : Prop :=
 | DInt n of T = ∅ & t = TInt n
@@ -379,8 +241,8 @@ case.
 - move=> ? -> -> _ /elem_of_singleton ->.
   rewrite tsize_TExp /= -ssrnat.plusE; lia.
 - move=> t1 ts1 t2 -> -> _.
-  case: (tsize_texp (TExp t1 ts1) t2); rewrite texpA ?is_exp_TExp //.
-  by move=> ?? /elem_of_union [] /elem_of_singleton ->.
+  case: (tsize_TExp_lt t1 ts1 t2) => ??.
+  by move=> /elem_of_union [] /elem_of_singleton ->.
 Qed.
 
 Fixpoint pterm_aux n t : iProp :=
@@ -696,1019 +558,94 @@ apply: (anti_symm _).
     by rewrite nonces_of_term_TExp.
 Qed.
 
-Lemma termT_int lvl n : ⊢ termT lvl (TInt n).
-Proof. by rewrite termT_eq. Qed.
-
-Lemma stermT_int n : ⊢ stermT Pub (TInt n).
-Proof. by rewrite /stermT termT_eq /=; iSplit; eauto. Qed.
-Hint Resolve stermT_int : typing.
-
-Lemma termT_aenc_pub_pub k t :
-  termT Pub (TKey Enc k) -∗
-  termT Pub t -∗
-  termT Pub (TEnc k t).
-Proof.
-rewrite [termT _ (TKey _ _)]termT_eq [termT _ (TEnc _ _)]termT_eq.
-iDestruct 1 as (lvl_enc lvl_dec) "[Hk %leq]".
-iIntros "Ht".
-iExists lvl_enc, lvl_dec; iSplit => //; iLeft; iSplit => //.
-by case: lvl_enc leq.
-Qed.
-
-Lemma termT_tag lvl n t :
-  termT lvl (Spec.tag n t) ⊣⊢ termT lvl t.
-Proof.
-by rewrite Spec.tag_eq termT_eq /= termT_eq bi.True_sep.
-Qed.
-
-Lemma termT_aenc_sec_pub N Φ lvl_k k t :
-  termT lvl_k (TKey Enc k) -∗
-  crypto_inv_meta N Φ -∗
-  termT Pub t -∗
-  □ Φ k t -∗
-  termT Pub (TEnc k (Spec.tag N t)).
-Proof.
-iIntros "#k_lo #pred #t_lo #inv".
-rewrite [termT _ (TEnc _ _)]termT_eq.
-rewrite [termT _ (TKey Enc _)]termT_eq.
-iDestruct "k_lo" as (lvl_enc lvl_dec) "[k_lo %leq]".
-iExists lvl_enc, lvl_dec; iSplit => //.
-iRight; iSplit => //; last first.
-  rewrite termT_tag.
-  iApply (sub_termT with "t_lo"); by case: (lvl_dec).
-by iExists N, t, Φ; eauto.
-Qed.
-
-Lemma stermTP lvl lvl' t :
-  stermT lvl t -∗ termT lvl' t -∗ ⌜lvl ⊑ lvl'⌝.
-Proof. by iIntros "[_ #min]". Qed.
-
-Lemma stermT_agree lvl lvl' t :
-  stermT lvl t -∗ stermT lvl' t -∗ ⌜lvl = lvl'⌝.
-Proof.
-iIntros "[#Ht #min] [#Ht' #min']".
-iPoseProof ("min" with "Ht'") as "%l1".
-iPoseProof ("min'" with "Ht") as "%l2".
-by case: lvl lvl' l1 l2 => [] // [] //.
-Qed.
-
-Lemma termT_to_list t ts lvl :
+Lemma pterm_to_list t ts :
   Spec.to_list t = Some ts →
-  termT lvl t -∗
-  [∗ list] t' ∈ ts, termT lvl t'.
+  pterm t -∗ [∗ list] t' ∈ ts, pterm t'.
 Proof.
 elim/term_ind': t ts => //=.
   by case=> // ts [<-] /=; iIntros "?".
 move=> t _ tl IH ts.
 case e: (Spec.to_list tl) => [ts'|] // [<-] /=.
-rewrite {1}termT_eq /=; iIntros "[??]"; iFrame.
+rewrite pterm_TPair /=; iIntros "[??]"; iFrame.
 by iApply IH.
 Qed.
 
-Lemma termT_of_list lvl ts :
-  termT lvl (Spec.of_list ts) ⊣⊢
-  [∗ list] t ∈ ts, termT lvl t.
+Lemma sterm_to_list t ts :
+  Spec.to_list t = Some ts →
+  sterm t -∗ [∗ list] t' ∈ ts, sterm t'.
+Proof.
+elim/term_ind': t ts => //=.
+  by case=> // ts [<-] /=; iIntros "?".
+move=> t _ tl IH ts.
+case e: (Spec.to_list tl) => [ts'|] // [<-] /=.
+rewrite sterm_TPair /=; iIntros "[??]"; iFrame.
+by iApply IH.
+Qed.
+
+Lemma pterm_of_list ts :
+  pterm (Spec.of_list ts) ⊣⊢
+  [∗ list] t ∈ ts, pterm t.
 Proof.
 rewrite Spec.of_list_eq.
-elim: ts => [|t ts IH]; first by rewrite termT_eq.
-by rewrite termT_eq /= IH.
+elim: ts => [|t ts IH]; first by rewrite pterm_TInt.
+by rewrite pterm_TPair /= IH bi.persistent_and_sep.
 Qed.
 
-Lemma stermT_pair lvl1 t1 lvl2 t2 :
-  stermT lvl1 t1 -∗
-  stermT lvl2 t2 -∗
-  stermT (lvl1 ⊔ lvl2) (TPair t1 t2).
+Lemma sterm_of_list ts :
+  sterm (Spec.of_list ts) ⊣⊢
+  [∗ list] t ∈ ts, sterm t.
 Proof.
-iIntros "[#type1 #min1] [#type2 #min2]"; iSplit.
-- rewrite (termT_eq (lvl1 ⊔ lvl2)).
-  iSplit; iApply sub_termT; try by [iApply "type1"|iApply "type2"];
-  by case: lvl1 lvl2=> [] [].
-- iIntros "!>" (lvl').
-  rewrite (termT_eq _ (TPair t1 t2)).
-  iIntros "[#type1' #type2']".
-  iPoseProof ("min1" with "type1'") as "%".
-  iPoseProof ("min2" with "type2'") as "%".
-  by iPureIntro; rewrite level_joinP; split.
+rewrite Spec.of_list_eq.
+elim: ts => [|t ts IH]; first by rewrite sterm_TInt.
+by rewrite sterm_TPair /= IH bi.persistent_and_sep.
 Qed.
 
-Lemma stermTS lvl t :
-  termT Pub t -∗
-  stermT lvl t -∗
-  ⌜lvl = Pub⌝.
+Lemma pterm_tag N t : pterm (Spec.tag N t) ⊣⊢ pterm t.
 Proof.
-iIntros "Ht1 [Ht2 #Hmin]".
-iSpecialize ("Hmin" with "Ht1").
-by case: lvl.
+by rewrite Spec.tag_eq pterm_TPair pterm_TInt bi.emp_and.
 Qed.
 
-Lemma termT_lvlP lvl t : termT lvl t -∗ ∃ lvl', stermT lvl' t.
+Lemma sterm_tag N t : sterm (Spec.tag N t) ⊣⊢ sterm t.
 Proof.
-elim/term_ind': t lvl=> [n|t1 IH1 t2 IH2|n|kt k IHk|k IHk t IHt|t IH|????] lvl /=;
-rewrite termT_eq /=.
-- iIntros "_"; iExists Pub; iApply stermT_int.
-- iIntros "[#type1 #type2]".
-  iDestruct (IH1 with "type1") as (lvl1) "type1'".
-  iDestruct (IH2 with "type2") as (lvl2) "type2'".
-  by iExists (lvl1 ⊔ lvl2); iApply stermT_pair.
-- iDestruct 1 as (lvl') "(#Hn & #Hmeta & %Hsub)".
-  iExists lvl'.
-  iSplit; first by rewrite termT_eq /=; eauto.
-  iIntros "!>" (lvl''); rewrite termT_eq /=.
-  iDestruct 1 as (lvl''') "# (Hn' & _ & %leq')".
-  by iPoseProof (atomicT_agree with "Hn' Hn") as "->".
-- iDestruct 1 as (lvl_enc lvl_dec) "[Hk _]".
-  rewrite keyT_eq; iDestruct "Hk" as "[??]".
-  by destruct kt; eauto.
-- iDestruct 1 as (lvl_enc lvl_dec) "# (Hk & Ht)".
-  iDestruct "Ht" as "[[-> Ht]|Ht]".
-    iExists Pub; rewrite stermT_eq keyT_eq stermT_eq.
-    iApply termT_aenc_pub_pub => //.
-    by iDestruct "Hk" as "[??]".
-  iDestruct "Ht" as "(#tP & Ht)".
-  iDestruct (IHt with "Ht") as (lvl') "Ht'".
-  case: lvl'.
-    iExists Pub; rewrite !stermT_eq /=.
-    rewrite [termT Pub (TEnc _ _)]termT_eq.
-    iExists lvl_enc, lvl_dec; iSplit => //.
-    case: lvl_enc; eauto.
-    iRight; iSplit => //.
-    by iApply (sub_termT with "Ht'").
-  rewrite stermT_eq; iDestruct "Ht'" as "[sec #pub]".
-  iExists (if lvl_dec is Sec then Pub else Sec).
-  rewrite stermT_eq; case: lvl_dec; last first.
-    rewrite (termT_eq _ (TEnc k t)).
-    iExists lvl_enc, Sec; iSplit => //.
-    by case: lvl_enc; eauto.
-  iSplit.
-    rewrite (termT_eq _ (TEnc k t)).
-    iExists lvl_enc, Pub; iSplit => //.
-    by iRight; eauto.
-  iIntros "!>"; rewrite (termT_eq _ (TEnc k t)).
-  iDestruct 1 as (lvl_enc' lvl_dec') "# (Hk' & Ht')".
-  iDestruct (keyT_agree with "Hk' Hk") as "[-> ->]".
-  iDestruct "Ht'" as "[[_ Ht']|Ht']".
-    by iApply "pub".
-  iDestruct "Ht'" as "(? & Ht')".
-  by iApply "pub".
-- iIntros "Ht"; iExists Pub; rewrite stermT_eq.
-  by rewrite [termT _ (THash t)]termT_eq.
-- by iIntros "[]".
+by rewrite Spec.tag_eq sterm_TPair sterm_TInt bi.emp_and.
 Qed.
 
-Lemma termT_TKey_swap l kt k :
-  termT l (TKey kt k) -∗
-  ∃ l', stermT l' (TKey (if kt is Enc then Dec else Enc) k).
+Lemma pterm_TEncE N Φ k t :
+  pterm (TEnc k (Spec.tag N t)) -∗
+  crypto_enc N Φ -∗
+  pterm t ∨
+  □ ▷ Φ k t ∧ sterm t ∧ □ (pterm (TKey Dec k) → pterm t).
 Proof.
-iIntros "Hk".
-iDestruct (termT_lvlP with "Hk") as (l') "Hk".
-rewrite stermT_TKey_eq.
-iDestruct "Hk" as (l_e l_d) "[Hk' ?]".
-iExists (if kt is Enc then l_d else l_e).
-rewrite stermT_TKey_eq.
-iExists l_e, l_d; iSplit => //.
-by case: (kt).
+iIntros "#Ht #HΦ"; rewrite pterm_TEnc pterm_tag.
+iDestruct "Ht" as "[[_ Ht] | Ht]"; first by eauto.
+rewrite sterm_TEnc sterm_tag.
+iDestruct "Ht" as "([??] & inv & ?)".
+iRight; iSplit; eauto; by iApply enc_inv_elim.
 Qed.
 
-Lemma termT_adec_pub N Φ k t :
-  termT Pub (TEnc k (Spec.tag N t)) -∗
-  crypto_inv_meta N Φ -∗
-  termT Pub t ∨ □ ▷ Φ k t ∗ termT Sec t.
-Proof.
-rewrite termT_eq; iIntros "#Ht #HΦ".
-iDestruct "Ht" as (lvl_enc lvl_dec) "# (Hk & Ht)".
-rewrite !termT_tag.
-iDestruct "Ht" as "[(?&?)|Ht]"; eauto.
-iDestruct "Ht" as "(inv & Ht)".
-iRight; iSplit; first by iApply enc_inv_elim.
-iApply (sub_termT with "Ht"); by case: lvl_dec.
-Qed.
-
-Lemma termT_adec_pub_sec N Φ k t :
-  termT Pub (TEnc k (Spec.tag N t)) -∗
-  crypto_inv_meta N Φ -∗
-  ∃ lvl, termT lvl t ∗ □ ▷ guarded (lvl = Sec) (Φ k t).
-Proof.
-iIntros "Ht Hpred".
-iPoseProof (termT_adec_pub with "Ht Hpred") as "[Ht|Ht]".
-- by iExists Pub; iSplit.
-- by iExists Sec; iDestruct "Ht" as "[??]"; iSplit.
-Qed.
-
-Lemma termT_adec_sec N Φ k lvl t :
-  stermT Sec (TKey Enc k) -∗
-  crypto_inv_meta N Φ -∗
-  termT lvl (TEnc k (Spec.tag N t)) -∗
-  termT Sec t ∗ □ ▷ Φ k t.
-Proof.
-iIntros "#Hk #HΦ #Ht".
-rewrite stermT_TKey_eq.
-iDestruct "Hk" as (? lvl_dec) "[Hk <-]".
-rewrite termT_eq.
-iDestruct "Ht" as (lvl_enc' lvl_dec') "(Hk' & Ht)".
-iDestruct (keyT_agree with "Hk' Hk") as "[-> ->]".
-iDestruct "Ht" as "[[% ?]|Ht]" => //.
-iDestruct "Ht" as "(#inv & Ht)"; rewrite termT_tag.
-iSplit.
-  iApply (sub_termT with "Ht"); by case: (_ ⊔ _).
-by iApply enc_inv_elim.
-Qed.
-
-Lemma termT_adec_sec_pub N Φ k t :
-  stermT Sec (TKey Enc k) -∗
-  crypto_inv_meta N Φ -∗
-  termT Pub (TKey Dec k) -∗
-  termT Pub (TEnc k (Spec.tag N t)) -∗
-  termT Pub t ∗ □ ▷ Φ k t.
-Proof.
-iIntros "#enc #HΦ #dec #Ht".
-iAssert (keyT Sec Pub k) as "{enc dec} Hk".
-  by rewrite keyT_eq [stermT Pub _]stermT_eq; iSplit.
-rewrite termT_eq.
-iDestruct "Ht" as (lvl_enc lvl_dec) "[Hk' Ht]".
-iDestruct (keyT_agree with "Hk' Hk") as "[-> ->]".
-iDestruct "Ht" as "[[% ?]|Ht]" => //.
-iDestruct "Ht" as "(#inv & Ht)".
-iSplit => //; first by rewrite termT_tag.
-by iApply enc_inv_elim.
-Qed.
-
-Lemma termT_adec_sec_pubG N Φ l k t :
-  stermT l (TKey Enc k) -∗
-  crypto_inv_meta N Φ -∗
-  termT Pub (TKey Dec k) -∗
-  termT Pub (TEnc k (Spec.tag N t)) -∗
-  termT Pub t ∗ □ ▷ guarded (l = Sec) (Φ k t).
-Proof.
-rewrite /guarded; case: decide => [->|_].
-  by iApply termT_adec_sec_pub.
-iIntros "_ _ #Hk #Ht".
-iAssert (stermT Pub (TKey Dec k)) as "{Hk} Hk".
-  by rewrite stermT_eq.
-rewrite stermT_TKey_eq.
-iDestruct "Hk" as (lvl_enc ?) "[Hk <-]".
-rewrite termT_eq.
-iDestruct "Ht" as (lvl_enc' lvl_dec') "[Hk' Ht]".
-iDestruct (keyT_agree with "Hk' Hk") as "[-> ->]".
-rewrite !termT_tag.
-iDestruct "Ht" as "[[??]|Ht]"; eauto.
-by iDestruct "Ht" as "(?&?)"; eauto.
-Qed.
-
-Lemma termT_aenc_pub_sec l N Φ k t :
-  termT  l (TKey Enc k) -∗
-  stermT Sec (TKey Dec k) -∗
-  crypto_inv_meta N Φ -∗
+Lemma pterm_TEncIS N Φ k t :
+  sterm (TKey Enc k) -∗
+  crypto_enc N Φ -∗
   □ Φ k t -∗
-  termT Sec t -∗
-  termT Pub (TEnc k (Spec.tag N t)).
+  sterm t -∗
+  □ (pterm (TKey Dec k) → pterm t) -∗
+  pterm (TEnc k (Spec.tag N t)).
 Proof.
-iIntros "#Henc #Hdec #HΦ #HΦt #Ht".
-iDestruct (termT_lvlP with "Henc") as (lvl') "{Henc} Henc".
-rewrite [termT _ (TEnc _ _)]termT_eq.
-iExists lvl', Sec; rewrite keyT_eq !termT_tag; iSplit; eauto.
-iRight; iSplit => //; iExists N, t, Φ; eauto.
+iIntros "#Henc #HΦ #HΦt #Ht #Hdecl".
+rewrite pterm_TEnc; iRight.
+rewrite sterm_TEnc sterm_tag pterm_tag.
+iSplit; first by rewrite sterm_TKey; eauto.
+iSplit; eauto.
+iExists N, t, Φ; eauto.
 Qed.
 
-Lemma termT_aenc_pub_secG k N Φ l t :
-  termT Pub (TKey Enc k) -∗
-  termT l t -∗
-  guarded (l = Sec) (stermT Sec (TKey Dec k)) -∗
-  crypto_inv_meta N Φ -∗
-  □ guarded (l = Sec) (Φ k t) -∗
-  termT Pub (TEnc k (Spec.tag N t)).
-Proof.
-iIntros "#Henc #Ht #Hdec #Hpred #HG"; case: l => /=.
-- by iApply termT_aenc_pub_pub; rewrite // termT_tag.
-- by iApply termT_aenc_pub_sec; rewrite // termT_tag.
-Qed.
-
-Lemma stermT_termT lvl t : stermT lvl t -∗ termT lvl t.
-Proof. by iDestruct 1 as "[??]". Qed.
-
-Lemma sub_termT_pub lvl t : termT Pub t -∗ termT lvl t.
-Proof. by iApply sub_termT. Qed.
-
-Definition term_inv t d : iProp :=
-  let '(lvl, _, _) := d in
-  ⌜atomic t⌝ ∗ stermT lvl t ∗
-  if lvl is Pub then published t ⊤ else emp.
-
-Global Instance term_inv_persistent t d : Persistent (term_inv t d).
-Proof.
-by case: t => *; case: d => [] [] [] * /=; apply _.
-Qed.
-
-Definition term_data_inv (td : term_data) : iProp :=
-  ([∗ map] t ↦ d ∈ td, term_inv t d)%I.
-
-Global Instance term_data_inv_persistent td : Persistent (term_data_inv td).
-Proof. by apply _. Qed.
-
-Definition crypto_inv :=
-  auth_inv crypto_name to_term_data' term_data_inv.
-
-Definition crypto_ctx :=
-  auth_ctx crypto_name cryptoN to_term_data' term_data_inv.
-
-Global Instance term_data'_cmra_total : CmraTotal term_data'UR.
-Proof. apply _. Qed.
-
-Global Instance term_data'_core_id (a : term_data'UR) : CoreId a.
-Proof.
-case: a => [] [] ???.
-apply _.
-Qed.
-
-(* MOVE *)
-Lemma auth_inv_acc' E (a : term_data'UR) :
-  ▷ auth_inv crypto_name to_term_data' term_data_inv ∗
-  crypto_own a ={E}=∗ ∃ t,
-    ⌜a ≼ to_term_data' t⌝ ∗ ▷ term_data_inv t ∗ ∀ u b,
-    ⌜(to_term_data' t, a) ~l~> (to_term_data' u, b)⌝ ∗
-    (crypto_own b -∗ ▷ term_data_inv u) ={E}=∗
-    ▷ auth_inv crypto_name to_term_data' term_data_inv ∗
-    crypto_own b.
-Proof using Type*.
-  iIntros "[Hinv Hγf]". rewrite /crypto_own /auth_inv /auth_own.
-  iDestruct "Hinv" as (t) "[>Hγa Hφ]".
-  iModIntro. iExists t.
-  iDestruct (own_valid_2 with "Hγa Hγf") as % [? ?]%auth_both_valid.
-  iSplit; first done. iFrame. iIntros (u b) "[% Hφ]".
-  iMod (own_update_2 with "Hγa Hγf") as "[Hγa Hγf]".
-  { eapply auth_update; eassumption. }
-  iPoseProof "Hγf" as "#Hγf".
-  iModIntro. iSplit => //. iExists u. iFrame. by iApply "Hφ".
-Qed.
-
-Lemma auth_acc' E (a : term_data'UR) :
-  ↑cryptoN ⊆ E →
-  crypto_ctx ∗ crypto_own a ={E,E ∖ ↑cryptoN}=∗
-  ∃ t, ⌜a ≼ to_term_data' t⌝ ∗
-       ▷ term_data_inv t ∗
-       (∀ u b,
-           ⌜(to_term_data' t, a) ~l~> (to_term_data' u, b)⌝ ∗
-           (crypto_own b -∗ ▷ term_data_inv u)
-           ={E ∖ ↑cryptoN,E}=∗ crypto_own b).
-Proof.
-  iIntros (?) "[#ctx Hγf]". rewrite /crypto_ctx /crypto_own /crypto_ctx /auth_ctx.
-  iInv "ctx" as "Hinv" "Hclose".
-  iMod (auth_inv_acc' with "[$Hinv $Hγf]") as (t) "(?&?&HclAuth)".
-  iModIntro. iExists t. iFrame. iIntros (u b) "H".
-  iMod ("HclAuth" $! u b with "H") as "(Hinv & ?)". by iMod ("Hclose" with "Hinv").
-Qed.
-(* /MOVE *)
-
-Lemma term_data_local_update td frag t lvl γ_pub γ_meta :
-  td !! t = None →
-  (to_term_data' td, frag) ~l~>
-  (to_term_data' (<[t := (lvl, γ_pub, γ_meta)]>td),
-   to_term_data' {[t := (lvl, γ_pub, γ_meta)]} ⋅ frag).
-Proof.
-move=> td_t.
-apply prod_local_update; last first.
-  rewrite /to_term_data' /= fmap_insert map_fmap_singleton.
-  rewrite insert_singleton_op ?lookup_fmap ?td_t //.
-  apply op_local_update_discrete => valid t'.
-  rewrite lookup_op.
-  destruct (decide (t' = t)) as [->|ne].
-    by rewrite lookup_singleton lookup_fmap td_t.
-  rewrite lookup_singleton_ne //.
-  by move: (valid t'); rewrite lookup_fmap left_id.
-apply prod_local_update; last first.
-  rewrite /to_term_data' /= fmap_insert map_fmap_singleton.
-  rewrite insert_singleton_op ?lookup_fmap ?td_t //.
-  apply op_local_update_discrete => valid t'.
-  rewrite lookup_op.
-  destruct (decide (t' = t)) as [->|ne].
-    by rewrite lookup_singleton lookup_fmap td_t.
-  rewrite lookup_singleton_ne //.
-  by move: (valid t'); rewrite lookup_fmap left_id.
-rewrite /to_term_data' /= fmap_insert map_fmap_singleton.
-rewrite insert_singleton_op ?lookup_fmap ?td_t //.
-apply op_local_update_discrete => valid t'.
-rewrite lookup_op.
-destruct (decide (t' = t)) as [->|ne].
-  by rewrite lookup_singleton lookup_fmap td_t.
-rewrite lookup_singleton_ne //.
-by move: (valid t'); rewrite lookup_fmap left_id.
-Qed.
-
-Lemma publish E lvl t Ts :
-  ↑cryptoN ⊆ E →
-  atomic t →
-  crypto_ctx -∗
-  stermT lvl t -∗
-  guarded (lvl = Sec) (unpublished t Ts) ={E}=∗
-  published t Ts.
-Proof.
-case: lvl => /=.
-- iIntros (? atomic_t) "#ctx #Ht _".
-  iMod (auth_empty crypto_name) as "#own0".
-  iMod (auth_acc' with "[ctx own0]") as (td) "{own0} (_ & #tdP & close)"; eauto.
-  destruct (td !! t) as [d|] eqn:td_t.
-  + case: d td_t => [] [] lvl' γ_pub γ_meta td_t.
-    iAssert (▷ term_inv t (lvl', γ_pub, γ_meta))%I as "#Ht'".
-    { iModIntro; rewrite /term_data_inv big_sepM_forall.
-      by iApply "tdP". }
-    iDestruct "Ht'" as "(_ & Ht' & publ)".
-    iAssert (▷ ⌜lvl' = Pub⌝)%I as ">->".
-    { iModIntro; iApply (stermT_agree with "Ht' Ht"). }
-    iDestruct "publ" as ">publ".
-    iMod ("close" $! td ε with "[]") as "_".
-      by iSplit => //; iIntros "_ !>".
-    iModIntro.
-    rewrite (union_difference_L Ts ⊤) // published_op.
-    by iDestruct "publ" as "[??]".
-  + iMod (own_alloc (coGset_pair_set ⊤)) as (γ_pub) "#publ" => //.
-    iMod (own_alloc (namespace_map_token ⊤)) as (γ_meta) "meta" => //.
-      apply namespace_map_token_valid.
-    pose (td' := <[t := (Pub, γ_pub, γ_meta)]>td).
-    pose (d'  := to_term_data' {[t := (Pub, γ_pub, γ_meta)]} ⋅ ε).
-    iMod ("close" $! td' d' with "[]") as "#own"; first iSplit.
-    * iPureIntro; by apply term_data_local_update.
-    * iIntros "#own !>".
-      rewrite /d' /crypto_own right_id auth_own_prod_3 /term_data_inv.
-      rewrite big_sepM_insert //; iSplit => //=.
-      do 2![iSplit => //].
-      iDestruct "own" as "(_ & ? & _)".
-      by iExists γ_pub; rewrite map_fmap_singleton; eauto.
-    rewrite /d' /crypto_own right_id auth_own_prod_3 !map_fmap_singleton.
-    iDestruct "own" as "(_ & ? & _)".
-    iAssert (published t ⊤) as "{publ} publ".
-      by iExists γ_pub; eauto.
-    rewrite (union_difference_L Ts ⊤) // published_op.
-    by iModIntro; iDestruct "publ" as "[??]".
-- iIntros (_ atomic_t) "#ctx #Ht unpubl".
-  iDestruct "unpubl" as (γ_pub) "[#own unpubl]".
-  iMod (own_update _ _ (coGset_pair_set Ts) with "unpubl") as "#publ".
-    apply: coGset_pair_alloc_update.
-  by iIntros "!>"; iExists γ_pub; iSplit.
-Qed.
-
-Lemma declare_nonce E1 E2 lvl a :
-  ↑cryptoN ⊆ E1 →
-  ↑cryptoN.@"nonce" ⊆ E2 →
-  crypto_ctx -∗
-  meta_token a E2 ={E1}=∗
-  stermT lvl (TNonce a) ∗
-  guarded (lvl = Sec) (unpublished (TNonce a) ⊤) ∗
-  crypto_meta_token (TNonce a) ⊤.
-Proof.
-iIntros (sub1 sub2) "#ctx Hmeta".
-iMod (auth_empty crypto_name) as "#own0".
-iMod (auth_acc' with "[ctx own0]")
-  as (td) "(_ & #tdP & close)"; eauto.
-pose (t := TNonce a); iAssert (▷ ⌜td !! t = None⌝)%I as "#>%undef".
-  case e: (td !! t) => [[] [] lvl' γ_pub_t γ_meta_t|] //=.
-  rewrite /term_data_inv big_sepM_forall.
-  iSpecialize ("tdP" $! _ _ e) => /=.
-  iDestruct "tdP" as "(_ & (tdP & _) & _)".
-  rewrite termT_eq /=.
-  iDestruct "tdP" as (?) "(_ & tdP & _)".
-  iModIntro.
-  by iDestruct (meta_meta_token with "Hmeta tdP") as "[]".
-pose (publ := if lvl is Pub then coGset_pair_set ⊤
-              else coGset_pair_unset ⊤).
-iMod (own_alloc publ) as (γ_pub) "publ" => //.
-  rewrite /publ; case: (lvl) => //.
-iMod (own_alloc (namespace_map_token ⊤)) as (γ_meta) "token" => //.
-  exact: namespace_map_token_valid.
-iMod (meta_set ⊤ a () (cryptoN.@"nonce") with "Hmeta") as "#l_nonce"; eauto.
-pose (d   := (lvl, γ_pub, γ_meta)).
-pose (td' := <[t := d]>td).
-iAssert (□ (⌜lvl = Pub⌝ -∗ own γ_pub (coGset_pair_set ⊤)))%I
-  with "[publ]" as "#publ'".
-  rewrite /publ; case: (lvl).
-  - by iDestruct "publ" as "#publ"; iIntros "!> _".
-  - by iIntros "!> %".
-iMod ("close" $! td' (to_term_data' {[t := d]} ⋅ ε) with "[]")
-  as "own"; first iSplit.
-- by iPureIntro; apply: term_data_local_update.
-- iIntros "#own !> {own0}".
-  rewrite /crypto_own right_id /term_data_inv big_sepM_insert //.
-  iSplit => //.
-  iSplit => //.
-  rewrite /to_term_data' !map_fmap_singleton /= /crypto_own.
-  rewrite auth_own_prod_3.
-  iDestruct "own" as "(own_lvl & own_pub & own_meta)".
-  iSplit; first iSplit.
-  + rewrite termT_eq /=.
-    iExists lvl; do 2![iSplit => //].
-  + iIntros "!>" (lvl').
-    rewrite termT_eq /=.
-    iDestruct 1 as (lvl'') "(own_lvl' & _ & %sub)".
-    by iDestruct (atomicT_agree with "own_lvl own_lvl'") as "<-".
-  + case: (lvl) => //.
-    iExists γ_pub; iSplit => //.
-    by iApply "publ'".
-rewrite /to_term_data' !map_fmap_singleton /= /crypto_own.
-rewrite right_id.
-iClear "own0"; rewrite auth_own_prod_3.
-iDestruct "own" as "# (Hlvl & Hpub & Hmeta)".
-iModIntro; iSplit.
-  iSplit; first by rewrite termT_eq; iExists lvl; eauto.
-  iIntros "!>" (lvl').
-  rewrite termT_eq.
-  iDestruct 1 as (lvl'') "(Ha & _ & %sub')".
-  by iDestruct (atomicT_agree with "Ha Hlvl") as "->".
-iSplitL "publ" => //.
-  rewrite /publ; case: (lvl) => //=.
-  by iExists γ_pub; iSplit.
-by iExists γ_meta; eauto.
-Qed.
-
-Lemma termT_atoms lvl t t' :
-  t' ∈ atoms t →
-  termT lvl t -∗ termT Sec t'.
-Proof.
-elim/term_ind': t lvl => //=.
-- move=> t1 IH1 t2 IH2 lvl t'_atom.
-  rewrite termT_eq; iIntros "[#Ht1 #Ht2]".
-  case/elem_of_union: t'_atom => t'_atom.
-  + by iApply IH1.
-  + by iApply IH2.
-- move=> a lvl /elem_of_singleton ->.
-  by apply sub_termT; case: lvl.
-- move=> kt k IH lvl /elem_of_singleton ->.
-  by apply sub_termT; case: lvl.
-- move=> k IHk t IHt lvl t'_atom.
-  iIntros "Ht".
-  rewrite termT_eq.
-  iDestruct "Ht" as (lvl_enc lvl_dec) "(_ & Ht)".
-  iDestruct "Ht" as "[(_ & Ht)|Ht]"; first by iApply IHt.
-  iDestruct "Ht" as "(_ & Ht)"; by iApply IHt.
-- by move=> ??????; rewrite termT_eq; iIntros "[]".
-Qed.
-
-Definition secret_terms (T T' : gset term) : iProp :=
-  □ (∀ t, ⌜t ∈ T'⌝ ∗-∗ ⌜t ∈ T⌝ ∧ stermT Sec t).
-
-Lemma secret_terms_sub T T' : secret_terms T T' -∗ ⌜T' ⊆ T⌝.
-Proof.
-rewrite elem_of_subseteq.
-iIntros "#secret" (t t_in).
-iDestruct ("secret" $! t) as "{secret} [secret _]".
-by iDestruct ("secret" with "[]") as "[??]" => //.
-Qed.
-
-Lemma secret_termsP T :
-  ([∗ set] t ∈ T, termT Sec t) -∗
-  ∃ T', secret_terms T T'.
-Proof.
-induction T as [|t T t_T IH] using set_ind_L.
-- iIntros "_"; iExists ∅.
-  iIntros "!>" (t); iSplit.
-  + iIntros (?); set_solver.
-  + iIntros "[%Ht _]"; case: H; set_solver.
-- rewrite big_sepS_insert //.
-  iIntros "[#Ht #HT]".
-  iDestruct (IH with "HT") as (T') "#HT'".
-  iDestruct (termT_lvlP with "Ht") as (lvl) "{Ht} Ht".
-  pose (T'' := if lvl is Sec then {[t]} : gset _ else ∅).
-  iExists (T'' ∪ T'); iIntros "!>" (t'); iSplit.
-  + iIntros "%t'_T'".
-    case/elem_of_union: t'_T' => t'_T'.
-      move: t'_T'; rewrite {}/T''; case: lvl; first set_solver.
-      move/elem_of_singleton=> ->.
-      iSplit => //.
-      iPureIntro; set_solver.
-    iDestruct ("HT'" $! t') as "{HT'} [HT' _]".
-    iDestruct ("HT'" $! t'_T') as "[%t'_T #Ht']".
-    iSplit => //.
-    iPureIntro; set_solver.
-  + iIntros "[%t'_T #Ht']".
-    case/elem_of_union: t'_T => [/elem_of_singleton ->|t'_T].
-      iDestruct (stermT_agree with "Ht Ht'") as "->".
-      by iPureIntro; set_solver.
-    iDestruct ("HT'" $! t') as "{HT'} [_ HT']".
-    rewrite elem_of_union; iRight.
-    iApply "HT'"; eauto.
-Qed.
-
-(* TODO Rename *)
-Lemma unpublished_secret T T' (P : term → iProp) :
-  secret_terms T T' -∗
-  ([∗ set] t ∈ T, □ (stermT Sec t -∗ P t)) -∗
-  [∗ set] t ∈ T', P t.
-Proof.
-move: T'.
-induction T as [|t T t_T IH] using set_ind_L.
-  iIntros (T') "secret _".
-  iPoseProof (secret_terms_sub with "secret") as "%sub".
-  assert (e : T' = ∅); first set_solver.
-  by rewrite e big_sepS_empty.
-iIntros (T') "secret unpub".
-destruct (decide (t ∈ T')) as [t_in|t_nin]; last first.
-  rewrite big_sepS_union; last set_solver.
-  iDestruct "unpub" as "[_ unpub]".
-  iApply (IH with "[secret]"); eauto.
-  iPoseProof "secret" as "#secret".
-  iIntros "!>" (t'); iDestruct ("secret" $! t') as "[s1 s2]".
-  iSplit.
-  - iIntros "%t'_T'".
-    iDestruct ("s1" with "[//]") as "[%t'_T ?]".
-    iSplit => //.
-    case/elem_of_union: t'_T => // /elem_of_singleton e.
-    congruence.
-  - iIntros "[%t'_T Ht']"; iApply "s2".
-    iSplit => //.
-    iPureIntro; set_solver.
-rewrite big_sepS_insert // (big_sepS_delete _ T' t) //.
-iPoseProof "secret" as "#secret".
-iDestruct "unpub" as "[u1 u2]".
-iSplitL "u1".
-  iApply "u1".
-  iDestruct ("secret" $! t) as "[s1 _]".
-  by iDestruct ("s1" with "[//]") as "[??]".
-iApply IH => //.
-iIntros "!>" (t'); iDestruct ("secret" $! t') as "[s1 s2]".
-iSplit.
-  iIntros ([t'_T' ne]%elem_of_difference).
-  iDestruct ("s1" with "[//]") as "{s1} [%s11 s12]".
-  iSplit => //.
-  iPureIntro; set_solver.
-iIntros "[%t'_T #?]".
-iDestruct ("s2" with "[]") as "%".
-  iSplit => //.
-  iPureIntro; set_solver.
-by iPureIntro; set_solver.
-Qed.
-
-Lemma stermT_atomicT t :
-  atomic t →
-  stermT Sec t -∗
-  atomicT Sec t.
-Proof.
-rewrite stermT_eq.
-case: t => //=.
-- move => a _.
-  rewrite !termT_eq.
-  iDestruct 1 as "[#sec #pub]".
-  iDestruct "sec" as (lvl) "(sec & ? & %leq)".
-  case: lvl leq => // _.
-  iDestruct ("pub" with "[]") as "[]".
-  by iExists Pub; do 2![iSplit => //].
-- move=> kt k _.
-  rewrite !termT_eq.
-  iDestruct 1 as "[#sec #pub]".
-  iDestruct "sec" as (lvl_enc lvl_dec) "[sec %leq]".
-  iDestruct "sec" as "[sec|(contra & -> & ->)]"; last first.
-    iDestruct ("pub" with "[]") as "[]".
-    iExists Pub, Pub; iSplit; last by case: (kt).
-    by iRight; repeat iSplit.
-  iDestruct "sec" as "(sec_enc & sec_dec & sec_k & #Hk)".
-  case: (kt) {leq}.
-  + case: lvl_enc => //.
-    iDestruct ("pub" with "[]") as "[]".
-    iExists Pub, lvl_dec; iSplit => //.
-    by iLeft; eauto.
-  + case: lvl_dec => //.
-    iDestruct ("pub" with "[]") as "[]".
-    iExists lvl_enc, Pub; iSplit => //.
-    by iLeft; eauto.
-Qed.
-
-Lemma big_sepS_exists `{Countable A, !EqDecision B} :
-  ∀ (Φ : A → B → iProp) (X : gset A),
-    ([∗ set] x ∈ X, ∃ y : B, Φ x y) -∗
-    ∃ m : gmap A B, ⌜dom _ m = X⌝ ∧ [∗ map] x↦y ∈ m, Φ x y.
-Proof.
-move=> Φ X.
-induction X as [|x X x_X IH] using set_ind_L.
-  by iIntros "_"; iExists ∅; iSplit; rewrite ?big_sepM_empty ?dom_empty_L.
-rewrite big_sepS_insert //.
-iIntros "[Hx HX]"; iDestruct "Hx" as (y) "Hx".
-iDestruct (IH with "HX") as (m) "[%dom_m Hm]".
-iExists (<[x := y]>m).
-rewrite dom_insert_L dom_m; iSplit => //.
-rewrite big_sepM_insert // -?(@not_elem_of_dom _ _ (gset A)) ?dom_m //.
-iFrame; iApply (big_sepS_mono with "Hf").
-Qed.
-
-Lemma big_opS_auth_own' `{!authG Σ A, !EqDecision B, !Countable B}
-  γ (g : B → A) (X : gset B) :
-  ([∗ set] x ∈ X, auth_own γ (g x)) ==∗
-  auth_own γ ([^op set] x ∈ X, g x).
-Proof.
-destruct (decide (X = ∅)) as [->|ne].
-  rewrite big_sepS_empty big_opS_empty; iIntros "_".
-  by iApply auth_empty.
-rewrite big_opS_auth_own //.
-by iIntros "? !>".
-Qed.
-
-Lemma big_opM_auth_own' `{!authG Σ A, !EqDecision B, !Countable B} {C}
-  γ (g : B → C → A) (m : gmap B C) :
-  ([∗ map] x↦y ∈ m, auth_own γ (g x y)) ==∗
-  auth_own γ ([^op map] x↦y ∈ m, g x y).
-Proof.
-destruct (decide (m = ∅)) as [->|ne].
-  rewrite big_sepM_empty big_opM_empty; iIntros "_".
-  by iApply auth_empty.
-rewrite big_opM_auth_own //.
-by iIntros "? !>".
-Qed.
-
-Lemma big_opS_pair {A1 : ucmraT} {A2 : ucmraT} `{!EqDecision B, !Countable B}
-  (g : B → prodUR A1 A2) (X : gset B) :
-  ([^op set] x ∈ X, g x) ≡
-  (([^op set] x ∈ X, (g x).1),
-   ([^op set] x ∈ X, (g x).2)).
-Proof.
-induction X as [|x X x_X IH] using set_ind_L.
-- by rewrite !big_opS_empty.
-- rewrite !big_opS_insert //.
-  by rewrite [X in X ≡ _]surjective_pairing /= IH.
-Qed.
-
-Lemma big_opM_pair {A1 : ucmraT} {A2 : ucmraT} `{!EqDecision B, !Countable B} {C}
-  (g : B → C → prodUR A1 A2) (m : gmap B C) :
-  ([^op map] x↦y ∈ m, g x y) ≡
-  (([^op map] x↦y ∈ m, (g x y).1),
-   ([^op map] x↦y ∈ m, (g x y).2)).
-Proof.
-induction m as [|x y m x_m IH] using map_ind.
-- by rewrite !big_opM_empty.
-- rewrite !big_opM_insert //.
-  by rewrite [X in X ≡ _]surjective_pairing /= IH.
-Qed.
-
-Lemma big_opM_fmap' `{!EqDecision A, !Countable A} {B} {C : cmraT}
-  (m : gmap A B) (f : B → C) :
-  ([^(@op (gmapUR _ _) _) map] x↦y ∈ m, {[x := f y]}) ≡ f <$> m.
-Proof.
-induction m as [|x y m x_m IH] using map_ind.
-- by rewrite !big_opM_empty fmap_empty.
-- rewrite big_opM_insert // IH.
-  move=> x'; rewrite lookup_op !lookup_fmap.
-  destruct (decide (x' = x)) as [->|ne].
-    by rewrite lookup_singleton x_m lookup_insert.
-  by rewrite lookup_singleton_ne // lookup_insert_ne // left_id.
-Qed.
-
-Lemma keyT_published lvl_enc lvl_dec k t :
-  t ∈ atoms k →
-  stermT Sec k -∗
-  keyT lvl_enc lvl_dec k -∗
-  published t {[TKey Enc k; TKey Dec k]}.
-Proof.
-iIntros (t_atom) "#Hk1 #[Hk2|Hk2]"; last first.
-  rewrite stermT_eq /=; iDestruct "Hk1" as "[_ #Hk1]".
-  iDestruct "Hk2" as "(Hk2 & _ & _)".
-  by iDestruct ("Hk1" with "Hk2") as "[]".
-iDestruct "Hk2" as "(_ & _ & Hpub & _ & _)".
-by rewrite big_sepS_delete //; iDestruct "Hpub" as "[??]".
-Qed.
-
-Lemma declare_sec_key E k t lvl_enc lvl_dec :
-  ↑cryptoN ⊆ E →
-  t ∈ atoms k →
-  crypto_ctx -∗
-  stermT Sec k -∗
-  stermT Sec t -∗
-  unpublished t {[TKey Enc k; TKey Dec k]} -∗
-  ([∗ set] t' ∈ atoms k ∖ {[t]}, published t' {[TKey Enc k; TKey Dec k]}) ={E}=∗
-  stermT lvl_enc (TKey Enc k) ∗
-  stermT lvl_dec (TKey Dec k) ∗
-  guarded (lvl_enc = Sec) (unpublished (TKey Enc k) ⊤) ∗
-  guarded (lvl_dec = Sec) (unpublished (TKey Dec k) ⊤) ∗
-  crypto_meta_token (TKey Enc k) ⊤ ∗
-  crypto_meta_token (TKey Dec k) ⊤.
-Proof.
-iIntros (sub t_atom) "#ctx #Hk #Ht unpubl #publ".
-iPoseProof (stermT_atomicT with "Ht") as "t_atomic" => //.
-  by apply: atomic_atom.
-iDestruct (big_sepS_exists with "publ") as (mγ) "[%dom_mγ publ']".
-rewrite big_sepM_sep.
-iDestruct "publ'" as "[own publ']".
-iMod (big_opM_auth_own' with "own") as "{own} own".
-rewrite !big_opM_pair /= !big_opM_unit big_opM_fmap'.
-iDestruct "unpubl" as (γ_pub_t) "[#t_pub unpubl]".
-rewrite {1}/atomicT /crypto_own.
-iCombine "t_atomic t_pub" as "{t_atomic} own_t".
-rewrite -auth_own_op -!pair_op !left_id right_id.
-iCombine "own own_t" as "{own_t} own".
-rewrite -auth_own_op -!pair_op !left_id.
-iMod (auth_acc' with "[ctx own]") as (td) "(%lb & #tdP & close)".
-- eauto.
-- iClear "t_pub"; eauto.
-move: lb; rewrite !pair_included; case=> [] [] Hlvl Hγ_pub _.
-move: Hlvl; rewrite lookup_included => /(_ t).
-rewrite /= lookup_fmap lookup_singleton => Ht.
-assert (is_Some (td !! t)) as [d td_t].
-  apply/fmap_is_Some.
-  by apply: is_Some_included (Ht) _; eauto.
-case: d td_t => [] [] lvl_t γ_pub_t' γ_meta_t td_t.
-move: Ht; rewrite td_t /= Some_included_total to_agree_included => e.
-apply leibniz_equiv in e; subst lvl_t.
-pose proof (Hγ_pub_t := transitivity (cmra_included_r _ _) Hγ_pub).
-pose proof (Hγ_pub_mγ := transitivity (cmra_included_l _ _) Hγ_pub).
-move: {Hγ_pub} Hγ_pub_t; rewrite lookup_included => /(_ t).
-rewrite /= lookup_fmap lookup_singleton td_t /=.
-rewrite Some_included_total to_agree_included => Hγ_pub_t.
-apply leibniz_equiv in Hγ_pub_t; subst γ_pub_t'.
-destruct (td !! TKey Enc k) as [d|] eqn:td_key_e.
-  iAssert (▷ False)%I with "[unpubl]" as ">[]"; iModIntro.
-  iAssert (unpublished t {[TKey Enc k; TKey Dec k]}) with "[unpubl]" as "unpubl".
-    by iExists γ_pub_t; iSplit.
-  rewrite /term_data_inv (big_sepM_forall _ td).
-  iPoseProof ("tdP" $! (TKey Enc k) with "[//]") as "decl".
-  case: d td_key_e => [] [] lvl_e γ_pub_e γ_meta_e td_key_e.
-  iDestruct "decl" as "(_ & #He & _)".
-  rewrite stermT_TKey_eq.
-  iDestruct "He" as (lvl_enc' lvl_dec') "[He <-]".
-  iPoseProof (keyT_published with "Hk He") as "{publ} publ"; eauto.
-  iPoseProof (own_publish_valid_2 with "publ unpubl") as "%valid".
-  rewrite coGset_pair_valid_eq /= left_id_L in valid.
-  set_solver.
-destruct (td !! TKey Dec k) as [d|] eqn:td_key_d.
-  iAssert (▷ False)%I with "[unpubl]" as ">[]"; iModIntro.
-  iAssert (unpublished t {[TKey Enc k; TKey Dec k]}) with "[unpubl]" as "unpubl".
-    by iExists γ_pub_t; iSplit.
-  rewrite /term_data_inv (big_sepM_forall _ td).
-  iPoseProof ("tdP" $! (TKey Dec k) with "[//]") as "decl".
-  case: d td_key_d => [] [] lvl_d γ_pub_d γ_meta_d td_key_d.
-  iDestruct "decl" as "(_ & #Hd & _)".
-  rewrite stermT_TKey_eq.
-  iDestruct "Hd" as (lvl_enc' lvl_dec') "[Hd <-]".
-  iPoseProof (keyT_published with "Hk Hd") as "{publ} publ"; eauto.
-  iPoseProof (own_publish_valid_2 with "publ unpubl") as "%valid".
-  rewrite coGset_pair_valid_eq /= left_id_L in valid.
-  set_solver.
-iMod (own_update _ _ (coGset_pair_set {[TKey Enc k; TKey Dec k]})
-        with "unpubl") as "#publ_t".
-  exact: coGset_pair_alloc_update.
-iAssert (published t {[TKey Enc k; TKey Dec k]}) as "{publ_t} publ_t".
-  by iExists γ_pub_t; eauto.
-pose (Ts_e := if lvl_enc is Pub then coGset_pair_set ⊤ else coGset_pair_unset ⊤).
-pose (Ts_d := if lvl_dec is Pub then coGset_pair_set ⊤ else coGset_pair_unset ⊤).
-iMod (own_alloc Ts_e) as (γ_pub_e) "pub_e" => //.
-  by rewrite /Ts_e; case: (lvl_enc).
-iMod (own_alloc Ts_d) as (γ_pub_d) "pub_d" => //.
-  by rewrite /Ts_d; case: (lvl_dec).
-iMod (own_alloc (namespace_map_token ⊤)) as (γ_meta_e) "meta_e" => //.
-  exact: namespace_map_token_valid.
-iMod (own_alloc (namespace_map_token ⊤)) as (γ_meta_d) "meta_d" => //.
-  exact: namespace_map_token_valid.
-pose (d_e := (lvl_enc, γ_pub_e, γ_meta_e)).
-pose (frag_e := {[TKey Enc k := d_e]} : gmap _ _).
-pose (d_d := (lvl_dec, γ_pub_d, γ_meta_d)).
-pose (frag_d := {[TKey Dec k := d_d]} : gmap _ _).
-pose (td' := <[TKey Enc k:=d_e]>(<[TKey Dec k:=d_d]>td)).
-set  frag := (singletonM _ _, op _ _, _).
-pose (frag' := to_term_data' {[TKey Enc k := d_e]} ⋅
-               (to_term_data' {[TKey Dec k := d_d]} ⋅ frag)).
-iAssert (crypto_own frag' -∗ stermT lvl_enc (TKey Enc k) ∗
-                             stermT lvl_dec (TKey Dec k))%I as "post".
-  rewrite /crypto_own 2!auth_own_op.
-  iIntros "#(own_e & own_d & _) {t_pub}".
-  rewrite /to_term_data' /= !map_fmap_singleton /=.
-  rewrite auth_own_prod_3.
-  iDestruct "own_e" as "(?&?&?)".
-  rewrite [auth_own crypto_name (singletonM _ _, singletonM _ _, _)]auth_own_prod_3.
-  iDestruct "own_d" as "(?&?&?)".
-  rewrite -keyT_eq.
-  iLeft.
-  do 3![iSplit => //].
-    rewrite (big_sepS_delete _ (atoms k)) //; iSplit => //.
-  by rewrite stermT_eq; iDestruct "Hk" as "[??]"; eauto.
-iAssert (⌜lvl_enc = Pub⌝ -∗ □ (crypto_own frag' -∗ published (TKey Enc k) ⊤))%I
-    with "[pub_e]" as "#pub_e'".
-  iIntros "->".
-  iPoseProof "pub_e" as "#pub_e".
-  rewrite /crypto_own 2!auth_own_op.
-  iIntros "!> (#own_e & _ & _) {post t_pub}".
-  rewrite /to_term_data' !map_fmap_singleton /= auth_own_prod_3.
-  iDestruct "own_e" as "(?&own_e&?)".
-  by iExists γ_pub_e; iSplit.
-iAssert (⌜lvl_dec = Pub⌝ -∗ □ (crypto_own frag' -∗ published (TKey Dec k) ⊤))%I
-    with "[pub_d]" as "#pub_d'".
-  iIntros "-> {post pub_e'}".
-  iPoseProof "pub_d" as "#pub_d".
-  rewrite /crypto_own 2!auth_own_op.
-  iIntros "!> (_ & #own_d & _) {t_pub}".
-  rewrite /to_term_data' !map_fmap_singleton /= auth_own_prod_3.
-  iDestruct "own_d" as "(?&own_d&?)".
-  by iExists γ_pub_d; iSplit.
-iMod ("close" $! td' frag' with "[]") as "#key_info"; first iSplit.
-- iPureIntro.
-  eapply transitivity; last first.
-    apply: term_data_local_update => //.
-    by rewrite lookup_insert_ne // td_key_e.
-  by apply: term_data_local_update => //.
-- iIntros "#own !> {t_pub}".
-  iDestruct ("post" with "own") as "{post} [??]".
-  rewrite /term_data_inv big_sepM_insert ?lookup_insert_ne //.
-  iSplit => //.
-    rewrite /=; do 2![iSplit => //].
-    case: (lvl_enc) => //.
-    by iDestruct ("pub_e'" with "[//] own") as "?".
-  rewrite big_sepM_insert ?lookup_insert_ne //.
-  iSplit => //.
-  rewrite /=; do 2![iSplit => //].
-  case: (lvl_dec) => //.
-  by iDestruct ("pub_d'" with "[//] own") as "?".
-iIntros "!> {pub_e' pub_d'}".
-iDestruct ("post" with "key_info") as "[??] {post t_pub}".
-rewrite /crypto_own !auth_own_op.
-iDestruct "key_info" as "(own_e & own_d & _)".
-rewrite /to_term_data' /= !map_fmap_singleton.
-rewrite auth_own_prod_3 /=; iDestruct "own_e" as "(?&?&?)".
-rewrite [auth_own _ (singletonM _ _, singletonM _ _, _)]auth_own_prod_3 /=.
-iDestruct "own_d" as "(?&?&?)".
-do 2![iSplit => //].
-iSplitL "pub_e" => //.
-  case: (lvl_enc) @Ts_e => //=.
-  by iExists γ_pub_e; iSplit.
-iSplitL "pub_d" => //.
-  case: (lvl_dec) @Ts_d => //=.
-  by iExists γ_pub_d; iSplit.
-by iSplitL "meta_e"; [iExists γ_meta_e|iExists γ_meta_d]; eauto.
-Qed.
-
-Lemma declare_pub_key k :
-  stermT Pub k -∗
-  stermT Pub (TKey Enc k) ∗
-  stermT Pub (TKey Dec k).
-Proof.
-iIntros "#Hk"; rewrite -keyT_eq.
-iRight.
-iSplit; first by iDestruct "Hk" as "[??]".
-by eauto.
-Qed.
-
-Lemma declare_key E k t lvl lvl_enc lvl_dec :
-  ↑cryptoN ⊆ E →
-  t ∈ atoms k →
-  lvl_enc ⊔ lvl_dec ⊑ lvl→
-  crypto_ctx -∗
-  stermT lvl k -∗
-  stermT lvl t -∗
-  guarded (lvl = Sec) (unpublished t {[TKey Enc k; TKey Dec k]}) -∗
-  guarded (lvl = Sec) (
-    [∗ set] t' ∈ atoms k ∖ {[t]}, published t' {[TKey Enc k; TKey Dec k]}) ={E}=∗
-  stermT lvl_enc (TKey Enc k) ∗
-  stermT lvl_dec (TKey Dec k) ∗
-  guarded (lvl_enc = Sec) (unpublished (TKey Enc k) ⊤) ∗
-  guarded (lvl_dec = Sec) (unpublished (TKey Dec k) ⊤) ∗
-  guarded (lvl = Sec) (crypto_meta_token (TKey Enc k) ⊤) ∗
-  guarded (lvl = Sec) (crypto_meta_token (TKey Dec k) ⊤).
-Proof.
-case: lvl => /=.
-  case: lvl_enc lvl_dec => [] // [] //= _ _ _.
-  iIntros "_ Hk _ _ _".
-  iDestruct (declare_pub_key with "Hk") as "[??]".
-  by iModIntro; iFrame.
-by iIntros (? ? ?); iApply declare_sec_key.
-Qed.
-
-Lemma atomic_atoms t : atomic t → atoms t = {[t]}.
-Proof. by case: t. Qed.
-
-Lemma crypto_own_valid_2 (td1 td2 : term_data') :
-  crypto_own td1 -∗
-  crypto_own td2 -∗
-  ✓ (td1 ⋅ td2).
-Proof.
-iIntros "#own1 #own2".
-iAssert (crypto_own (td1 ⋅ td2)) as "own".
-  by rewrite /crypto_own auth_own_op; iSplit.
-iApply (auth_own_valid with "own").
-Qed.
-
-Lemma unpublished_op t Ts1 Ts2 :
-  Ts1 ## Ts2 →
-  unpublished t (Ts1 ⋅ Ts2) ⊣⊢ unpublished t Ts1 ∗ unpublished t Ts2.
-Proof.
-move=> disj; apply (anti_symm _).
-- iDestruct 1 as (γ) "[#H1 H2]".
-  rewrite coGset_pair_unset_union //.
-  by iDestruct "H2" as "[H21 H22]"; iSplitL "H21"; iExists γ; iSplit.
-- iIntros "[H1 H2]".
-  iDestruct "H1" as (γ1) "[#H11 H12]".
-  iDestruct "H2" as (γ2) "[#H21 H22]".
-  iPoseProof (crypto_own_valid_2 with "H11 H21") as "%valid".
-  case: valid => [] /= [] _ /= valid _.
-  rewrite singleton_op singleton_valid in valid *.
-  move=> /agree_op_invL' ->.
-  iExists γ2; iSplit => //.
-  by rewrite coGset_pair_unset_union // own_op; iFrame.
-Qed.
-
-Lemma unpublished_difference t Ts1 Ts2 :
-  Ts1 ⊆ Ts2 →
-  unpublished t Ts2 ⊣⊢ unpublished t Ts1 ∗ unpublished t (Ts2 ∖ Ts1).
-Proof.
-move=> sub.
-rewrite {1}(_ : Ts2 = Ts1 ∪ (Ts2 ∖ Ts1)) ?unpublished_op //; first set_solver.
-rewrite [_ ∪ _]comm_L difference_union_L. set_solver.
-Qed.
-
-Lemma termT_hash l t : termT l (THash t) ⊣⊢ termT Sec t.
-Proof. by rewrite termT_eq. Qed.
+Lemma pterm_TEncIP k t :
+  pterm (TKey Enc k) -∗
+  pterm t -∗
+  pterm (TEnc k t).
+Proof. by iIntros "? ?"; rewrite pterm_TEnc; eauto. Qed.
 
 End Resources.
 
-Arguments crypto_name {Σ _}.
-Arguments crypto_inv {Σ _ _}.
-Arguments crypto_ctx {Σ _ _}.
+Arguments crypto_enc_name {Σ _}.
+Arguments crypto_enc {Σ _ _}.
