term.v
@@ -356,6 +356,31 @@ Definition tdec c k t :=
   | None => None
   end.
 
+
+Definition texp t1 t2 :=
+  if t1 is TExp' base exp _ then
+    TExp base (t2 :: map fold_term exp)
+  else TInt 0.
+
+Lemma texpA t1 ts1 t2 : texp (TExp t1 ts1) t2 = TExp t1 (t2 :: ts1).
+Proof.
+rewrite /texp {1}unlock /= fold_wf_termE normalize_unfold1 normalize_unfoldn.
+rewrite unfold_termK.
+apply: TExp_perm.
+rewrite seq.perm_cons -{2}[ts1](seq.mapK unfold_termK).
+by rewrite seq.perm_map // path.perm_sort.
+Qed.
+
+Lemma unfold_exp t1 t2 :
+  unfold_term (texp t1 t2) = PreTerm.exp (unfold_term t1) (unfold_term t2).
+Proof.
+case: t1 => //= t1 ts1 /(ssrbool.elimT ssrbool.andP) [wf_ts1 ?].
+rewrite unfold_TExp /=; congr PreTerm.PTExp.
+apply: (ssrbool.elimT (perm_sort_leP _ _ _ _)); rewrite seq.perm_cons.
+rewrite -[@List.map]/@seq.map -seq.map_comp seq.map_id_in //= => {}t1 in_ts1.
+by rewrite fold_termK // (ssrbool.elimT seq.allP wf_ts1).
+Qed.
+
 End Spec.
 
 Arguments repr_term /.
